theories/Operational/Awkernel/MinimalProjection.v
@@ -4,6 +4,9 @@ From RocqSched Require Import Semantics.Schedule.
 From RocqSched Require Import Operational.Common.State.
 From RocqSched Require Import Operational.Common.Trace.
 From RocqSched Require Import Operational.Common.Projection.
+From RocqSched Require Import Operational.Common.Invariants.
+From RocqSched Require Import Operational.Common.Execution.
+From RocqSched Require Import Operational.Common.ProjectionLemmas.
 Import ListNotations.
 
 Record AwkernelState : Type := mkAwkernelState {
@@ -27,6 +30,30 @@ Definition awk_projected_running
     (m : nat) (tr : AwkernelTrace) (j : JobId) (t : Time) : Prop :=
   projected_running m (awk_to_op_trace tr) j t.
 
+Record awk_execution (m : nat) : Type := mkAwkExecution {
+  awk_ex_trace : AwkernelTrace;
+  awk_ex_init : Prop;
+  awk_ex_stepwise : trace_stepwise (awk_to_op_trace awk_ex_trace);
+  awk_ex_struct_inv : forall t, op_struct_inv m (awk_to_op_state (awk_ex_trace t));
+}.
+
+Arguments awk_ex_trace {m} _ _.
+Arguments awk_ex_init {m} _.
+Arguments awk_ex_stepwise {m} _ _.
+Arguments awk_ex_struct_inv {m} _ _.
+
+Definition awk_to_execution {m} (ex : awk_execution m) : execution m :=
+  mkExecution
+    m
+    (awk_to_op_trace (awk_ex_trace ex))
+    (awk_ex_init ex)
+    (awk_ex_stepwise ex)
+    (awk_ex_struct_inv ex).
+
+Definition awk_trace_sound
+    (jobs : JobId -> Job) (m : nat) (ex : awk_execution m) : Prop :=
+  execution_projection_sound jobs m (awk_to_execution ex).
+
 Lemma awk_project_schedule_eq :
   forall tr t c,
     awk_project_schedule tr t c = awk_current (tr t) c.
@@ -44,4 +71,17 @@ Proof.
   unfold awk_projected_running, awk_to_op_trace.
   rewrite projected_running_iff_current.
   tauto.
+Qed.
+
+Lemma awk_trace_sound_implies_valid_schedule :
+  forall jobs m ex,
+    awk_trace_sound jobs m ex ->
+    valid_schedule jobs m (awk_project_schedule (awk_ex_trace ex)).
+Proof.
+  intros jobs m ex Hsound.
+  unfold awk_trace_sound in Hsound.
+  change (valid_schedule jobs m
+            (project_schedule (ex_trace (awk_to_execution ex)))).
+  apply execution_projection_sound_implies_valid_schedule.
+  exact Hsound.
 Qed.
