theories/Operational/Common/Execution.v
@@ -1,0 +1,28 @@
+From Stdlib Require Import List Bool Arith Arith.PeanoNat Lia.
+From RocqSched Require Import Foundation.Base.
+From RocqSched Require Import Operational.Common.Trace.
+From RocqSched Require Import Operational.Common.Step.
+From RocqSched Require Import Operational.Common.Invariants.
+
+Definition trace_stepwise (tr : OpTrace) : Prop :=
+  forall t, exists ev, op_step (tr t) ev (tr (S t)).
+
+Record execution (m : nat) : Type := mkExecution {
+  ex_trace : OpTrace;
+  ex_init : Prop;
+  ex_stepwise : trace_stepwise ex_trace;
+  ex_struct_inv : forall t, op_struct_inv m (ex_trace t);
+}.
+
+Arguments ex_trace {m} _ _.
+Arguments ex_init {m} _.
+Arguments ex_stepwise {m} _ _.
+Arguments ex_struct_inv {m} _ _.
+
+Lemma execution_trace_step :
+  forall m (ex : execution m) t,
+    exists ev, op_step (ex_trace ex t) ev (ex_trace ex (S t)).
+Proof.
+  intros m ex t.
+  exact (ex_stepwise ex t).
+Qed.
