theories/Operational/Common/StepLemmas.v
@@ -1,0 +1,213 @@
+From Stdlib Require Import List Bool Arith Arith.PeanoNat Lia.
+From RocqSched Require Import Foundation.Base.
+From RocqSched Require Import Operational.Common.State.
+From RocqSched Require Import Operational.Common.Step.
+From RocqSched Require Import Operational.Common.Invariants.
+Import ListNotations.
+
+Lemma remove_job_in :
+  forall j x xs,
+    In x (remove_job j xs) ->
+    In x xs /\ x <> j.
+Proof.
+  intros j x xs.
+  induction xs as [|y ys IH]; simpl.
+  - intros [].
+  - destruct (Nat.eqb y j) eqn:Hy.
+    + intros Hrem.
+      specialize (IH Hrem) as [Hin_tail Hneq].
+      split; [right; exact Hin_tail|exact Hneq].
+    + intros [->|Hrem].
+      * split.
+        -- left. reflexivity.
+        -- apply Nat.eqb_neq in Hy. exact Hy.
+      * specialize (IH Hrem) as [Hin' Hneq].
+        split; [right; exact Hin'|exact Hneq].
+Qed.
+
+Lemma remove_job_not_in :
+  forall j xs,
+    ~ In j (remove_job j xs).
+Proof.
+  intros j xs Hin.
+  apply remove_job_in in Hin as [_ Hneq].
+  contradiction.
+Qed.
+
+Lemma remove_job_preserves_NoDup :
+  forall j xs,
+    NoDup xs ->
+    NoDup (remove_job j xs).
+Proof.
+  intros j xs Hnd.
+  induction Hnd as [|x xs Hnotin Hnd IH]; simpl.
+  - constructor.
+  - destruct (Nat.eqb x j) eqn:Hxj.
+    + exact IH.
+    + constructor.
+      * intros Hin.
+        apply remove_job_in in Hin as [Hin _].
+        contradiction.
+      * exact IH.
+Qed.
+
+Lemma op_job_running_current :
+  forall st j,
+    op_job_running st j ->
+    exists c, op_current st c = Some j.
+Proof.
+  intros st j [c Hcur].
+  exists c. exact Hcur.
+Qed.
+
+Definition op_step_sound_pre (st : OpState) (ev : OpEvent) : Prop :=
+  match ev with
+  | EvWakeup j => ~ In j (op_runnable st) /\ ~ op_job_running st j
+  | _ => True
+  end.
+
+Lemma add_runnable_preserves_struct_inv :
+  forall m st j,
+    op_struct_inv m st ->
+    ~ In j (op_runnable st) ->
+    ~ op_job_running st j ->
+    op_struct_inv m (add_runnable j st).
+Proof.
+  intros m st j Hinv Hnotin Hnotrunning.
+  destruct Hinv as [Hdup Hnodup Hsep].
+  constructor.
+  - exact Hdup.
+  - simpl. constructor; assumption.
+  - intros c j' Hlt Hcur.
+    simpl.
+    intros [Heq|Hin].
+    + subst j'.
+      apply Hnotrunning.
+      exists c. exact Hcur.
+    + eapply Hsep; eauto.
+Qed.
+
+Lemma clear_current_and_request_preserves_struct_inv :
+  forall m st j,
+    op_struct_inv m st ->
+    op_struct_inv m (clear_current_and_request j st).
+Proof.
+  intros m st j Hinv.
+  destruct Hinv as [Hdup Hnodup Hsep].
+  constructor.
+  - intros j' c1 c2 Hlt1 Hlt2.
+    intros Hcur1 Hcur2.
+    simpl in Hcur1, Hcur2.
+    destruct (op_current st c1) as [k1|] eqn:Hc1; try discriminate.
+    destruct (Nat.eqb k1 j) eqn:Ek1; try discriminate.
+    destruct (op_current st c2) as [k2|] eqn:Hc2; try discriminate.
+    destruct (Nat.eqb k2 j) eqn:Ek2; try discriminate.
+    inversion Hcur1; inversion Hcur2; subst.
+    eapply Hdup; eauto.
+  - simpl. apply remove_job_preserves_NoDup. exact Hnodup.
+  - intros c j' Hlt.
+    intros Hcur Hin.
+    simpl in Hcur.
+    destruct (op_current st c) as [k|] eqn:Hc; try discriminate.
+    destruct (Nat.eqb k j) eqn:Ek; try discriminate.
+    inversion Hcur; subst.
+    apply remove_job_in in Hin as [Hin' _].
+    eapply Hsep; eauto.
+Qed.
+
+Lemma set_need_resched_preserves_struct_inv :
+  forall m st c b,
+    op_struct_inv m st ->
+    op_struct_inv m (set_need_resched c b st).
+Proof.
+  intros m st c b [Hdup Hnodup Hsep].
+  constructor; simpl; assumption.
+Qed.
+
+Lemma dispatch_target_not_in_remove_job :
+  forall j xs,
+    ~ In j (remove_job j xs).
+Proof.
+  apply remove_job_not_in.
+Qed.
+
+Lemma dispatch_other_not_in_remove_job :
+  forall j j' xs,
+    j' <> j ->
+    ~ In j' xs ->
+    ~ In j' (remove_job j xs).
+Proof.
+  intros j j' xs Hneq Hnotin Hin.
+  apply remove_job_in in Hin as [Hin _].
+  contradiction.
+Qed.
+
+Lemma dispatch_preserves_struct_inv :
+  forall m st c j,
+    op_struct_inv m st ->
+    In j (op_runnable st) ->
+    op_current st c = None ->
+    c < m ->
+    op_struct_inv
+      m
+      (clear_need_resched c
+         (mkOpState
+            (fun c' => if Nat.eqb c' c then Some j else op_current st c')
+            (remove_job j (op_runnable st))
+            (op_need_resched st))).
+Proof.
+  intros m st c j Hinv Hin Hjnone Hltc.
+  destruct Hinv as [Hdup Hnodup Hsep].
+  constructor.
+  - intros j' c1 c2 Hlt1 Hlt2.
+    simpl.
+    destruct (Nat.eqb c1 c) eqn:Ec1, (Nat.eqb c2 c) eqn:Ec2;
+      intros Hcur1 Hcur2.
+    + apply Nat.eqb_eq in Ec1.
+      apply Nat.eqb_eq in Ec2.
+      lia.
+    + apply Nat.eqb_eq in Ec1.
+      apply Nat.eqb_neq in Ec2.
+      subst c1.
+      inversion Hcur1; subst j'.
+      exfalso.
+      eapply (Hsep c2 j); eauto.
+    + apply Nat.eqb_neq in Ec1.
+      apply Nat.eqb_eq in Ec2.
+      subst c2.
+      inversion Hcur2; subst j'.
+      exfalso.
+      eapply (Hsep c1 j); eauto.
+    + eapply Hdup; eauto.
+  - simpl. apply remove_job_preserves_NoDup. exact Hnodup.
+  - intros c' j' Hlt'.
+    intros Hcur Hin'.
+    simpl in Hcur.
+    destruct (Nat.eqb c' c) eqn:Ecc.
+    + apply Nat.eqb_eq in Ecc. subst c'.
+      inversion Hcur; subst j'.
+      exact (dispatch_target_not_in_remove_job j (op_runnable st) Hin').
+    + apply Nat.eqb_neq in Ecc.
+      eapply Hsep; eauto.
+      eapply remove_job_in in Hin' as [Hin'' _].
+      exact Hin''.
+Qed.
+
+Lemma op_step_preserves_struct_inv :
+  forall m st ev st',
+    op_struct_inv m st ->
+    op_step_sound_pre st ev ->
+    op_step st ev st' ->
+    (forall c j, ev = EvDispatch c j -> c < m) ->
+    op_struct_inv m st'.
+Proof.
+  intros m st ev st' Hinv Hpre Hstep Hdispatch_lt.
+  inversion Hstep; subst; clear Hstep.
+  - destruct Hpre as [Hnotin Hnotrunning].
+    apply add_runnable_preserves_struct_inv; assumption.
+  - apply clear_current_and_request_preserves_struct_inv; assumption.
+  - apply clear_current_and_request_preserves_struct_inv; assumption.
+  - apply set_need_resched_preserves_struct_inv; assumption.
+  - eapply dispatch_preserves_struct_inv; eauto using Hdispatch_lt.
+  - exact Hinv.
+Qed.
